More tree specifications.

lib/Lib.Seq.fsti
@@ -2,6 +2,8 @@ module Lib.Seq
 
 module Seq = FStar.Seq
 
+unfold let op_String_Access #a = Seq.index #a
+
 let unsnoc (#a: Type) (s: Seq.seq a{
   Seq.length s > 0
 }): Tot (res: Seq.seq a{
@@ -11,7 +13,41 @@ let unsnoc (#a: Type) (s: Seq.seq a{
 }) =
   Seq.slice s 0 (Seq.length s - 1)
 
-unfold let op_String_Access #a = Seq.index #a
+module List = FStar.List.Tot
+
+let no_dup (#a: Type{hasEq a}) (s: Seq.seq a) =
+  forall (x: a). {:pattern Seq.count x s} Seq.mem x s ==> Seq.count x s == 1
+
+let disjoint (#a: Type{hasEq a}) (s1 s2: Seq.seq a) =
+  forall (x: a). {:pattern (Seq.mem x s1); (Seq.mem x s2)}
+    (Seq.mem x s1 ==> Seq.mem x s2 = false) /\
+    (Seq.mem x s2 ==> Seq.mem x s1 = false)
+
+let disjoint_comm (#a: Type{hasEq a}) (s1 s2: Seq.seq a): Lemma
+  (requires disjoint s1 s2)
+  (ensures disjoint s2 s1)
+  [SMTPat (disjoint s1 s2)] = ()
+
+let no_dup_append (#a: Type{hasEq a}) (s1 s2: Seq.seq a): Lemma
+  (requires no_dup s1 /\ no_dup s2 /\ disjoint s1 s2)
+  (ensures no_dup (Seq.append s1 s2))
+  [SMTPat (no_dup s1); SMTPat (no_dup s2); SMTPat (disjoint s1 s2)] =
+  match Seq.length s1 with
+  | 0 ->
+    Seq.lemma_empty s1;
+    Seq.append_empty_l s2
+  | _ -> Seq.lemma_append_count s1 s2
+
+let no_dup_append' (#a: Type{hasEq a}) (s1 s2: Seq.seq a): Lemma
+  (requires no_dup (Seq.append s1 s2))
+  (ensures no_dup s1 /\ no_dup s2 /\ disjoint s1 s2)
+  [SMTPat (no_dup (Seq.append s1 s2))] =
+  match Seq.length s1 with
+  | 0 ->
+    Seq.lemma_empty s1;
+    Seq.append_empty_l s2
+  | _ ->
+    Seq.lemma_append_count s1 s2
 
 let slice_empty (#a: Type) (s: Seq.seq a) (len: nat): Lemma
   (requires len == 0)
